leetcode/preorderTraversal.dfy
@@ -1,0 +1,205 @@
+include "./invertTree.dfy"
+
+module PreorderTraversal {
+    import opened InvertBinaryTree
+    method SetToSeq<T>(s: set<T>) returns (xs: seq<T>)
+      ensures multiset(s) == multiset(xs)
+    {
+      xs := [];
+      var left: set<T> := s;
+      while left != {}
+        invariant multiset(left) + multiset(xs) == multiset(s)
+      {
+        var x :| x in left;
+        left := left - {x};
+        xs := xs + [x];
+      }
+    }
+
+    function children(node: TreeNode): set<TreeNode> 
+        reads node, node.repr
+    {
+        (if node.right != null then {node.right} else {}) + 
+        (if node.left != null then {node.left} else {})
+    }
+    function childStack(node: TreeNode?): seq<TreeNode> 
+        reads node
+    {
+        if node == null then [] else
+        (if node.right != null then [node.right] else []) + 
+        (if node.left != null then [node.left] else [])
+    }
+
+    function mapNodes(ss: seq<TreeNode>): seq<int> 
+        reads set i | 0 <= i < |ss| :: ss[i]
+    {
+        if ss == [] then [] else [ss[0].val]+mapNodes(ss[1..])
+    }    
+
+  predicate compare(a: TreeNode, b: TreeNode)
+    reads a, b
+  {
+    a.val <= b.val
+  }
+
+lemma ThereIsAMinimum(s: set<TreeNode>)
+  requires s != {}
+  ensures exists x :: x in s && forall y :: y in s ==> compare(x, y)
+{
+  var x :| x in s;
+  if s == {x} {
+    // obviously, x is the minimum
+  } else {
+    // The minimum in s might be x, or it might be the minimum
+    // in s - {x}. If we knew the minimum of the latter, then
+    // we could compare the two.
+    // Let's start by giving a name to the smaller set:
+    var s' := s - {x};
+    // So, s is the union of s' and {x}:
+    assert s == s' + {x};
+    // The following lemma call establishes that there is a
+    // minimum in s'.
+    ThereIsAMinimum(s');
+  }
+}
+
+// lemma ThereIsAMinimumTwo(s: set<int>)
+//   requires s != {}
+//   ensures exists x :: x in s && forall y :: y in s ==> x <= y
+// {
+//   var x :| x in s;
+//   if s == {x} {
+//   } else {
+//     var s' := s - {x};
+//     assert s == s' + {x};
+//     ThereIsAMinimumTwo(s');
+//   }
+// }
+
+//     ghost function gmapNodeSet(ss: set<TreeNode>): set<int> 
+//         reads ss
+//         ensures forall xx :: xx in gmapNodeSet(ss) ==> exists s :: s in ss && s.val == xx
+//     {
+//         if ss == {} then 
+//             {}
+//         else 
+//             var s :| s in ss;
+//             {s.val}+gmapNodeSet(ss - {s})
+//     }    
+
+// lemma ThereIsAMinimumG(s: set<TreeNode>)
+//   requires s != {}
+//   ensures exists x :: x in gmapNodeSet(s) && forall y :: y in gmapNodeSet(s) ==> x<= y
+// {
+//     var xx :| xx in s  && gmapNodeSet(s) == {xx.val}+gmapNodeSet(s-{xx});
+//     var x :| x in gmapNodeSet(s) && xx.val == x;
+//   if s == {xx} {
+//     // obviously, x is the minimum
+//   } else {
+//     var s' := s - {xx};
+//     assert s == s' + {xx};
+//     ThereIsAMinimumG(s');
+//     var mm :| mm in gmapNodeSet(s') && forall y :: y in gmapNodeSet(s') ==> mm <= y;
+//     if x <= mm {
+//       assert x in gmapNodeSet(s) && forall y :: y in gmapNodeSet(s) ==> x <= y;
+//     }else{
+//       assert mm in gmapNodeSet(s) && forall y :: y in gmapNodeSet(s) ==> mm <= y;
+        
+//     }
+//   }
+// }
+
+    predicate uniqueNodes(ss: set<TreeNode>)
+      reads ss
+    {
+      forall x,y :: x in ss && y in ss && x != y ==> x.val != y.val 
+    }
+
+
+    // function mapNodeSet(ss: set<TreeNode>): set<int> 
+    //   reads ss
+    //   requires uniqueNodes(ss)
+    // {
+    //     if ss == {} then 
+    //         {}
+    //     else 
+    //       ThereIsAMinimum(ss);
+    //       // ThereIsAMinimumG(ss);
+    //       var s :| s in ss && forall ys :: ys in ss ==> compare(s, ys);
+    //       {s.val}+mapNodeSet(ss - {s})
+    // }    
+    
+    method Traverse(root: TreeNode) returns (result: seq<TreeNode>)
+        requires root.Valid()
+        decreases *
+    {
+        var stack := [root];
+        var i := 0;
+        result := [];
+        var visited: set<TreeNode> := {};
+        var visiteds: seq<TreeNode> := [];
+        var unvisited: set<TreeNode> := root.repr;
+        var parents: seq<TreeNode> := [];
+        var parentIndices: seq<int> := [];
+        while |stack| > 0 
+            invariant |parents| == |parentIndices|
+            decreases *
+        {
+            print "i: ", i, "\n";
+            print "pre ", "result ", mapNodes(result), " \n";
+            print "pre ", "stack ", mapNodes(stack), " \n";
+            print "pre ", "parents ", mapNodes(parents), " \n";
+            print "pre ", "parentIndices ", parentIndices, " \n";
+            print "pre ", "visited ", mapNodes(visiteds), " \n";
+            var current := stack[|stack|-1];
+            var stack' := childStack(current);
+            if |stack'| > 0 {
+                parentIndices := parentIndices + [i];
+                parents := parents + [current];
+            }
+            stack := stack[..|stack|-1]+stack';
+            result := result + [current];
+            visited := visited + {current};
+            visiteds := visiteds + [current];
+            unvisited := unvisited-{current};
+            if |parents| > 0 { 
+              var childnodes := SetToSeq(children(parents[|parents|-1]));
+              print "children, ", mapNodes(childnodes);
+            }
+            if |parents| > 0 && children(parents[|parents|-1]) <= visited {
+                parents := parents[..|parents|-1];
+                parentIndices := parentIndices[..|parentIndices|-1];
+            }
+
+            print "post ", "result ", mapNodes(result), " \n";
+            print "post ", "stack ", mapNodes(stack), " \n";
+            print "post ", "parents ", mapNodes(parents), " \n";
+            print "post ", "parentIndices ", parentIndices, " \n";
+            print "post ", "visited ", mapNodes(visiteds), " \n";
+            i := i + 1;
+        }
+        return result;
+    }
+
+    method Main() 
+      decreases *
+    {
+        var u := new TreeNode(20, null, null);
+        var v := new TreeNode(21, null, null);
+        var l := new TreeNode(12, u, v);
+        var m := new TreeNode(13, null, null);
+        var h := new TreeNode(8, l, m);
+        var o := new TreeNode(14, null, null);
+        var p := new TreeNode(15, null, null);
+        var i := new TreeNode(9, o, p);
+        var d := new TreeNode(4, h, i);
+        var e := new TreeNode(5, null, null);
+        var b := new TreeNode(2, d, e);
+        var c := new TreeNode(3, null, null);
+        var a := new TreeNode(1, b, c);
+        var flat := Traverse(a);
+        print mapNodes(flat), "\n";
+        print mapNodes(PreorderTraversal(a)), "\n";
+
+    }
+}
